Update to Coq 8.10

Instances/Except.v
@@ -19,11 +19,22 @@ Section except_maybe.
     | _ => x
     end.
   Hint Unfold trycatch_maybe : soundness.
+
+  Lemma trycatch_maybe_throw_left : ∀ A (x : Maybe A),
+    trycatch_maybe None x = x.
+  Proof. simple_solve. Qed.
+
+  Lemma trycatch_maybe_throw_right : ∀ A (x : Maybe A),
+    trycatch_maybe x None = x.
+  Proof. simple_solve. Qed.
+
   Instance except_maybe : Except Maybe :=
   {
     throw := @None;
     trycatch := @trycatch_maybe;
-  }. all: solve_monad. Defined.
+    trycatch_throw_left := trycatch_maybe_throw_left;
+    trycatch_throw_right := trycatch_maybe_throw_right;
+  }.
 End except_maybe.
 
 Section except_maybeT.
@@ -53,8 +64,9 @@ Section except_maybeT.
     trycatch_maybeT x throw_maybeT = x.
   Proof.
     autounfold with soundness. intros.
+    replace x with (bindM (M:=M) x pure) at 2.
+    f_equal; ext; destruct x0; reflexivity.
     rewrite <- (bind_id_right (M:=M)). f_equal.
-    ext. destruct x0; reflexivity.
   Qed.
 
   Instance except_maybeT : Except (MaybeT M) :=
@@ -79,36 +91,55 @@ Section except_maybeAT.
       | JustOrNoneA a => pure (JustOrNoneA a) (* should be a join_op *)
       | NoneA => my
       end).
-  
   Arguments trycatch_maybeAT [_].
   Hint Unfold throw_maybeAT trycatch_maybeAT : soundness.
+
+  Lemma trycatch_maybeAT_throw_left : ∀ A (x : MaybeAT M A),
+    trycatch_maybeAT throw_maybeAT x = x.
+  Proof. simple_solve. Qed.
+  
+  Lemma trycatch_maybeAT_throw_right : ∀ A (x : MaybeAT M A),
+    trycatch_maybeAT x throw_maybeAT = x.
+  Proof. 
+    intros. unfold trycatch_maybeAT. rewrite <- (@bind_id_right M inst).
+    f_equal; ext. destruct x0; reflexivity.
+  Qed.
 
   Instance except_maybeAT : Except (MaybeAT M) :=
     {
       throw := @throw_maybeAT;
       trycatch := trycatch_maybeAT;
-    }. 1,3: solve_monad.
-      intros. unfold trycatch_maybeAT. 
-      rewrite <- (@bind_id_right M inst). f_equal. simple_solve.
-    Defined.
+      trycatch_throw_left := trycatch_maybeAT_throw_left;
+      trycatch_throw_right := trycatch_maybeAT_throw_right;
+    }. 
 End except_maybeAT.
 
 Section except_stateT.
   Context {M : Type -> Type} `{inst_m : Monad M} 
     `{inst_e : @Except M inst_m}.
+  Context {S : Type}.
 
-  Definition throw_stateT {S} A : StateT S M A := fun _ => throw.
+  Definition throw_stateT {A} : StateT S M A := fun _ => throw.
 
-  Definition trycatch_stateT {S A} (a b : StateT S M A) : StateT S M A := 
+  Definition trycatch_stateT {A} (a b : StateT S M A) : StateT S M A := 
     fun s => trycatch (a s) (b s).
   Hint Unfold throw_stateT trycatch_stateT : soundness.
 
-  Instance except_stateT (S : Type) : Except (StateT S M) :=
+  Lemma trycatch_stateT_throw_left : ∀ A (x : StateT S M A),
+    trycatch_stateT throw_stateT x = x.
+  Proof. simple_solve. Qed.
+
+  Lemma trycatch_stateT_throw_right : ∀ A (x : StateT S M A),
+    trycatch_stateT x throw_stateT = x.
+  Proof. simple_solve. Qed.
+
+  Instance except_stateT : Except (StateT S M) :=
   {
-    throw := @throw_stateT S;
-    trycatch := @trycatch_stateT S;
-  }. all: solve_monad. 
-  Qed.
+    throw := @throw_stateT;
+    trycatch := @trycatch_stateT;
+    trycatch_throw_left := trycatch_stateT_throw_left;
+    trycatch_throw_right := trycatch_stateT_throw_right;
+  }. 
 End except_stateT.
 
 Global Instance except_abstract_state : Except AbstractState.
